Rename [dlist]->[node] and [dlisthead]->[dll]

ind/DListLowInd.fst
@@ -9,63 +9,63 @@ open FStar.Modifies
 
 unopteq
 (** Node of a doubly linked list *)
-type dlist (t:Type0) = {
+type node (t:Type0) = {
   (* forward link *)
-  flink: gpointer_or_null (dlist t);
+  flink: gpointer_or_null (node t);
   (* backward link *)
-  blink: gpointer_or_null (dlist t);
+  blink: gpointer_or_null (node t);
   (* payload *)
   p: t;
 }
 
 unopteq
 (** Doubly linked list head *)
-type dlisthead (t:Type0) ={
-  lhead: gpointer_or_null (dlist t);
-  ltail: gpointer_or_null (dlist t);
-  nodes: erased (list (gpointer (dlist t)));
+type dll (t:Type0) ={
+  lhead: gpointer_or_null (node t);
+  ltail: gpointer_or_null (node t);
+  nodes: erased (list (gpointer (node t)));
 }
 
-type nonempty_dlisthead t = (h:dlisthead t{is_not_null h.lhead /\ is_not_null h.ltail})
+type nonempty_dll t = (h:dll t{is_not_null h.lhead /\ is_not_null h.ltail})
 
 (** Initialize an element of a doubly linked list *)
-val empty_entry: #t:Type -> payload:t -> dlist t
+val empty_entry: #t:Type -> payload:t -> node t
 let empty_entry #t payload =
   { flink = null ; blink = null ; p = payload }
 
 (** Initialize a doubly linked list head *)
-val empty_list: #t:Type -> dlisthead t
+val empty_list: #t:Type -> dll t
 let empty_list #t =
   { lhead = null ; ltail = null ; nodes = hide [] }
 
 unfold let (.[]) (s:list 'a) (n:nat{n < length s}) = index s n
 
 logic
-let dlist_is_valid' (#t:Type) (h0:heap) (n:dlist t) : GTot Type0 =
+let node_is_valid' (#t:Type) (h0:heap) (n:node t) : GTot Type0 =
   not_aliased n.flink n.blink
 
 // logic
-let dlist_is_valid (#t:Type) (h0:heap) (n:gpointer (dlist t)) : GTot Type0 =
+let node_is_valid (#t:Type) (h0:heap) (n:gpointer (node t)) : GTot Type0 =
   h0 `contains` n /\
-  dlist_is_valid' h0 (n@h0)
+  node_is_valid' h0 (n@h0)
 
 logic
-let ( |> ) (#t:Type) (a:dlist t) (b:gpointer (dlist t)) : GTot Type0 =
+let ( |> ) (#t:Type) (a:node t) (b:gpointer (node t)) : GTot Type0 =
   a.flink ==$ b
 
 logic
-let ( <| ) (#t:Type) (a:gpointer (dlist t)) (b: dlist t) : GTot Type0 =
+let ( <| ) (#t:Type) (a:gpointer (node t)) (b: node t) : GTot Type0 =
   b.blink ==$ a
 
 irreducible
-let ( =|> ) (#t:Type) (a:gpointer (dlist t)) (b:gpointer (dlist t)) : ST unit
+let ( =|> ) (#t:Type) (a:gpointer (node t)) (b:gpointer (node t)) : ST unit
     (requires (fun h0 ->
          h0 `contains` a /\ h0 `contains` b /\
          not_aliased00 a b /\
          not_aliased0 b (a@h0).blink))
     (ensures (fun h1 _ h2 ->
          modifies_1 a h1 h2 /\
-         dlist_is_valid h2 a /\
+         node_is_valid h2 a /\
          (a@h1).p == (a@h2).p /\
          (a@h1).blink == (a@h2).blink /\
          b@h1 == b@h2 /\
@@ -73,14 +73,14 @@ let ( =|> ) (#t:Type) (a:gpointer (dlist t)) (b:gpointer (dlist t)) : ST unit
   a := { !a with flink = of_non_null b }
 
 irreducible
-let ( <|= ) (#t:Type) (a:gpointer (dlist t)) (b:gpointer (dlist t)) : ST unit
+let ( <|= ) (#t:Type) (a:gpointer (node t)) (b:gpointer (node t)) : ST unit
     (requires (fun h0 ->
          h0 `contains` a /\ h0 `contains` b /\
          not_aliased00 a b /\
          not_aliased0 a (b@h0).flink))
     (ensures (fun h1 _ h2 ->
          modifies_1 b h1 h2 /\
-         dlist_is_valid h2 b /\
+         node_is_valid h2 b /\
          a@h1 == a@h2 /\
          (b@h1).p == (b@h2).p /\
          (b@h1).flink == (b@h2).flink /\
@@ -88,22 +88,22 @@ let ( <|= ) (#t:Type) (a:gpointer (dlist t)) (b:gpointer (dlist t)) : ST unit
   b := { !b with blink = of_non_null a }
 
 irreducible
-let ( !=|> ) (#t:Type) (a:gpointer (dlist t)) : ST unit
+let ( !=|> ) (#t:Type) (a:gpointer (node t)) : ST unit
     (requires (fun h0 -> h0 `contains` a))
     (ensures (fun h1 _ h2 ->
          modifies_1 a h1 h2 /\
-         dlist_is_valid h2 a /\
+         node_is_valid h2 a /\
          (a@h1).p == (a@h2).p /\
          (a@h1).blink == (a@h2).blink /\
          (a@h2).flink == null)) =
   a := { !a with flink = null }
 
 irreducible
-let ( !<|= ) (#t:Type) (a:gpointer (dlist t)) : ST unit
+let ( !<|= ) (#t:Type) (a:gpointer (node t)) : ST unit
     (requires (fun h0 -> h0 `contains` a))
     (ensures (fun h1 _ h2 ->
          modifies_1 a h1 h2 /\
-         dlist_is_valid h2 a /\
+         node_is_valid h2 a /\
          (a@h1).p == (a@h2).p /\
          (a@h1).flink == (a@h2).flink /\
          (a@h2).blink == null)) =
@@ -113,4 +113,4 @@ unfold let (~.) (#t:Type) (a:t) : Tot (erased (list t)) = hide ([a])
 unfold let (^+) (#t:Type) (a:t) (b:erased (list t)) : Tot (erased (list t)) = elift2 Cons (hide a) b
 unfold let (+^) (#t:Type) (a:erased (list t)) (b:t) : Tot (erased (list t)) = elift2 append a (hide [b])
 
-/// A "fragment" is a list of "piece"s, such that each piece is an "almost valid" dlisthead
+/// A "fragment" is a list of "piece"s, such that each piece is an "almost valid" dll
